re

src/pca.lean
@@ -11,7 +11,6 @@ infix ` ↓= `:50 := λ x y, x = some y
 prefix `↓`:80 := some
 
 abbreviation defined : option α → bool := option.is_some
-
 def partial_magma.mmul [partial_magma α] : option α → option α → option α
 | ↓x ↓y := x ⬝ y
 | _ _   := none
@@ -20,7 +19,7 @@ instance pm_mul [partial_magma α] : has_mul (option α) := {mul := @partial_mag
 @[simp] lemma partial_magma.none_l [partial_magma α] (p : option α) : none * p = none := option.cases_on p rfl (λ a, rfl)
 @[simp] lemma partial_magma.none_r [partial_magma α] (p : option α) : p * none = none := option.cases_on p rfl (λ a, rfl)
 
-lemma defined_l [partial_magma α] (p q : option α) : defined (p * q) → defined p :=
+lemma defined_l [partial_magma α] {p q : option α} : defined (p * q) → defined p :=
 begin
   contrapose,
   assume (h0 : ¬ defined p),
@@ -29,7 +28,7 @@ begin
   simp,
 end
 
-lemma defined_r [partial_magma α] (p q : option α) : defined (p * q) → defined q :=
+lemma defined_r [partial_magma α] {p q : option α} : defined (p * q) → defined q :=
 begin
   contrapose,
   assume (h0 : ¬ defined q),
@@ -38,7 +37,7 @@ begin
   simp,
 end
 
-abbreviation tot [partial_magma α] (a : α) : Prop := ∀ x : α, defined (a ⬝ x) = tt
+def tot [partial_magma α] (a : α) : Prop := ∀ x : α, defined (↓a * ↓x) = tt
 
 /- Partial Combinatory Algebra -/
 class pca (α : Type u) extends partial_magma α :=
@@ -46,7 +45,7 @@ class pca (α : Type u) extends partial_magma α :=
 (ktot : ∀ x, defined (k ⬝ x))
 (k_constant : ∀ x y : α, k ⬝ x * y = x)
 (s : α)
-(stot : ∀ x y : α, defined (s ⬝ x * y))
+(stot' : ∀ x y : α, defined (s ⬝ x * y))
 (s_substitution : ∀ x y z : α, s ⬝ x * y * z = (x ⬝ z) * (y ⬝ z))
 
 def pca.equiv [partial_magma α] (a b : option α) : Prop := ∀ x : α, a * ↓x = b * ↓x
@@ -55,7 +54,7 @@ infix ` ≃ `:50 := pca.equiv
 namespace pca
 
 def const [pca α] (x : α) : α := option.get (ktot x)
-def subst [pca α] (x y : α) : α := option.get (stot x y)
+def subst [pca α] (x y : α) : α := option.get (stot' x y)
 notation `𝐤` := const
 notation `𝐬` := subst
 
@@ -66,61 +65,58 @@ notation `𝐬` := subst
 
 def i [pca α] : α := 𝐬 k k
 @[simp] lemma i_ident [pca α] (a : α) : ↓i * ↓a = ↓a := by { unfold i, simp, }
+lemma itot [pca α] : tot (i : α) := by { intros x, simp, refl, }
 
-lemma stot0 [pca α] (a : α) : defined (↓s * ↓a) := defined_l (↓s * ↓a) a (stot _ _)
+lemma stot [pca α] : tot (s : α) := λ a, defined_l (stot' a a)
 
-def subst0 [pca α] (x : α) : α := option.get (stot0 x)
-notation `𝐬₀` := subst0
+def subst' [pca α] (x : α) : α := option.get (stot x)
+notation `𝐬'` := subst'
 
 inductive lambda (α : Type u) [pca α]
 | var : ℕ → lambda
 | com : α → lambda
 | app : lambda → lambda → lambda
+prefix `#` := lambda.var
+prefix `&`:max := lambda.com
 instance lambda_mul (α : Type u) [pca α] : has_mul (lambda α) := ⟨lambda.app⟩
 
-open lambda
-
 def lam [pca α] (n : ℕ) :lambda α → lambda α
-| (var m) := if n = m then com i else com k * var m
-| (com c) := com k * com c
-| (l * k) := (com s) * (lam l) * (lam k)
+| #m := if n = m then &i else &k * #m
+| &c := &k * &c
+| (l * k) := &s * (lam l) * (lam k)
 notation `Λ`x`,` := lam x 
 
 def expr [pca α] : lambda α → option α
-| (var x) := ↓k
-| (com c) := ↓c
+| #x := ↓k
+| &c := ↓c
 | (l * k) := (expr l) * (expr k)
 
-lemma lambda_defined [c : pca α] : ∀ (n : ℕ) (e : lambda α), defined (expr (Λ n, e) : option α)
-| n (var e) := begin
+lemma lambda_defined [c : pca α] (n : ℕ) : ∀ (e : lambda α), defined (expr (Λ n, e) : option α)
+| #e := begin
     cases (eq.decidable n e),
     { simp[lam, expr, if_neg h], exact rfl, },
     { simp[lam, expr, if_pos h], exact rfl, },
   end
-| n (com c) := ktot c
-| n (l * m) := begin
+| &c := ktot c
+| (l * m) := begin
     simp [lam, expr], 
-    let a := option.get (lambda_defined n l),
-    let b := option.get (lambda_defined n m),
+    let a := option.get (lambda_defined l),
+    let b := option.get (lambda_defined m),
     have ha : expr (Λ n, l) = ↓a, { simp },
     have hb : expr (Λ n, m) = ↓b, { simp },
     rw [ha, hb],
-    exact stot a b
+    exact stot' a b
   end
 
 notation n` ↦ `l := option.get (lambda_defined n l)
 
 namespace recursion
 
-def d [pca α] : α := 0 ↦ Λ 1, (var 0 * var 0 * var 1)
+def d [pca α] : α := 0 ↦ Λ 1, (#0 * #0 * #1)
+def dd [pca α] : lambda α := Λ 0, (Λ 1, (#0 * #0 * #1))
 
 lemma dtot [pca α] (f : α) : defined (d ⬝ f) :=
-begin
-  have e : d ⬝ f = expr (Λ 0, (com f * com f * var 0)),
-  { change (d ⬝ f) with (↓d * ↓f), unfold d, simp [lam, expr], },
-  rw e,
-  exact (lambda_defined 0 _),
-end
+by { change (d ⬝ f) with (↓d * ↓f), unfold d, simp [lam, expr], exact rfl, }
 
 lemma diagonal [pca α] (f x : α) : d ⬝ f * x = f ⬝ f * x :=
 begin
@@ -129,13 +125,13 @@ begin
     ...        = f ⬝ f * ↓x   : by { unfold d, simp [lam, expr], refl, }
 end
 
-def v [pca α] : α := 0 ↦ Λ 1, (var 0 * (com d * var 1))
-def n [pca α] : α := 0 ↦ com d * (com v * var 0)
+def v [pca α] : α := 0 ↦ Λ 1, (#0 * (&d * #1))
+def n [pca α] : α := 0 ↦ &d * (&v * #0)
 
 theorem recursion [pca α] (f : α) : n ⬝ f ≃ f * (n ⬝ f) :=
 begin
   intros x,
-  let vf := (0 ↦ com f * (com d * var 0)),  
+  let vf := (0 ↦ &f * (&d * #0)),  
   have hv : ↓v * ↓f = ↓vf, { unfold v, simp [lam, expr], },
   have nf_dvf : ↓n * ↓f = ↓d * ↓vf,  { unfold n, unfold v, simp [lam, expr], },
   calc
@@ -148,7 +144,7 @@ end
 
 theorem ntot [pca α] (f : α) : defined (↓n * ↓f) :=
 begin
-  let vf := (0 ↦ com f * (com d * var 0)),  
+  let vf := (0 ↦ &f * (&d * #0)),  
   have hv : ↓v * ↓f = ↓vf, { unfold v, simp [lam, expr], },
   have nf_dvf : ↓n * ↓f = ↓d * ↓vf,  { unfold n, unfold v, simp [lam, expr], },
   rw nf_dvf,
@@ -160,94 +156,5 @@ end recursion
 def fixpoint [pca α] : α := recursion.n
 def recursion  [pca α] (f x : α) : ↓fixpoint * ↓f * ↓x = f * (↓fixpoint * ↓f) * ↓x := recursion.recursion f x
 def fixpoint_of [pca α] (f : α) : α := option.get (recursion.ntot f)
-
-namespace calculation
-
-def pair [pca α] : α := 0 ↦ Λ 1, (Λ 2, (var 2 * var 0 * var 1))
-notation `⟪`a`, `b`⟫` := 0 ↦ var 0 * com a * com b
-def π₀ [pca α] : α := 0 ↦ var 0 * com k
-def π₁ [pca α] : α := 0 ↦ var 0 * (com k * com i)
-
-lemma pair_h [pca α] (a b : α) : ↓pair * ↓a * ↓b = ↓⟪a, b⟫ :=
-begin
-  calc
-    ↓pair * ↓a * ↓b = expr (Λ 0, (Λ 1, (Λ 2, (var 2 * var 0 * var 1)))) * ↓a * ↓b
-      : by { unfold pair, simp, }
-    ...             = expr (Λ 0, (var 0 * com a * com b))
-      : by {simp [lam, expr, if_neg (show 2 ≠ 0, from dec_trivial), if_neg (show 2 ≠ 1, from dec_trivial)], }
-    ...             = ↓⟪a, b⟫
-      : by { simp, },
-end
-
-lemma pair_pi0 [pca α] (a b : α) : ↓π₀ * ↓⟪a, b⟫ = ↓a := by { unfold π₀, simp [lam, expr], }
-lemma pair_pi1 [pca α] (a b : α) : ↓π₁ * ↓⟪a, b⟫ = ↓b := by { unfold π₁, simp [lam, expr], }
-
-end calculation
-
-inductive prec [pca α] : set α
-| k : prec k
-| s : prec s
-| mul {a b c} : ↓a * ↓b = ↓c → prec a → prec b → prec c 
-notation `ℰ` := prec
-
-def recursive [pca α] : set α := {x | prec x ∧ tot x}
-notation `ℛ` := recursive
-#check ℛ
-
-lemma prec.const [pca α] {a : α} : a ∈ (ℰ : set α) → 𝐤 a ∈ (ℰ : set α) :=
-begin
-  assume h : a ∈ ℰ,
-  have l0 : ↓k * ↓a = ↓𝐤 a, { simp, },
-  show 𝐤 a ∈ ℰ, from prec.mul l0 prec.k h,
-end
-
-lemma prec.subst [pca α] {a b : α}
-: a ∈ (ℰ : set α) → b ∈ (ℰ : set α) → 𝐬 a b ∈ (ℰ : set α) :=
-begin
-  assume (ha : a ∈ ℰ) (hb : b ∈ ℰ),
-  have l0 : ↓s * ↓a = ↓𝐬₀ a, { unfold subst0, simp, },
-  have l1 : 𝐬₀ a ∈ (ℰ : set α), from prec.mul l0 prec.s ha,
-  have l2 : ↓𝐬₀ a * ↓b = ↓𝐬 a b, { unfold subst0, simp, },
-  show 𝐬 a b ∈ ℰ, from prec.mul l2 l1 hb,
-end
-
-lemma prec.i [pca α] : i ∈ (ℰ : set α) := prec.subst prec.k prec.k
-
-def K [pca α] : set α := {x : α | defined (↓x * ↓x)}
-def re_set [pca α] (A : set α) : Prop := ∃ e : α, e ∈ (ℰ : set α) ∧ A = {x | defined (↓e * ↓x)}
-
-lemma neg_p_iff_negp (P : Prop) : ¬(P ↔ ¬P) := 
-begin
-  rintros ⟨h₀, h₁⟩,
-  have h₂ : ¬ P := λ p, h₀ p p,
-  exact h₂ (h₁ h₂),
-end
-
-lemma K_re [pca α] : re_set (K : set α) :=
-begin
-  use (0 ↦ var 0 * var 0),
-  have h : ∀ x : α, expr (Λ 0, (var 0 * var 0)) * ↓x = ↓x * ↓x, { intros x, simp [lam, expr], },
-  split,
-  { simp [lam, expr],
-    show 𝐬 i i ∈ ℰ, from prec.subst prec.i prec.i, },
-  apply set.ext,
-  intros x,
-  split,
-  { assume xK, simp, rw h x, exact xK, },
-  { unfold K, simp, assume xh, rw ← h x, exact xh, },
-end
-
-lemma compl_K_nre [pca α] : ¬ re_set (Kᶜ : set α) :=
-begin
-  rintro ⟨e, h⟩,
-  apply neg_p_iff_negp (e ∈ (K : set α)),
-  split,
-  { assume eK : e ∈ K,
-    show e ∈ (Kᶜ : set α), { rw h.2, simp, exact eK, }, },
-  { assume nKc : e ∉ K,
-    have eKc : e ∈ (Kᶜ : set α) := nKc,
-    show e ∈ K, { unfold K, simp, rw h.2 at eKc, exact eKc, }, },
-end
-
 
 end pca
