src/combinator.lean
@@ -1,0 +1,33 @@
+import pca
+
+namespace pca
+
+universe variable u
+variables {α : Type u}
+
+namespace combinator
+
+def pair [pca α] : α := 0 ↦ Λ 1, (Λ 2, (#2 * #0 * #1))
+notation `⟪`a`, `b`⟫` := 0 ↦ #0 * (&a) * &b
+def π₀ [pca α] : α := 0 ↦ #0 * &k
+def π₁ [pca α] : α := 0 ↦ #0 * (&k * &i)
+
+lemma pair_h [pca α] (a b : α) : ↓pair * ↓a * ↓b = ↓⟪a, b⟫ :=
+begin
+  calc
+    ↓pair * ↓a * ↓b = expr (Λ 0, (Λ 1, (Λ 2, (#2 * #0 * #1)))) * ↓a * ↓b
+      : by { unfold pair, simp, }
+    ...             = expr (Λ 0, (#0 * &a * &b))
+      : by {simp [lam, pca.expr, if_neg (show 2 ≠ 0, from dec_trivial), if_neg (show 2 ≠ 1, from dec_trivial)], }
+    ...             = ↓⟪a, b⟫
+      : by { simp, },
+end
+
+lemma pair_pi0 [pca α] (a b : α) : ↓π₀ * ↓⟪a, b⟫ = ↓a := by { unfold π₀, simp [lam, pca.expr], }
+lemma pair_pi1 [pca α] (a b : α) : ↓π₁ * ↓⟪a, b⟫ = ↓b := by { unfold π₁, simp [lam, pca.expr], }
+
+def top [pca α] : α := 0 ↦ Λ 1, (#0)
+def bot [pca α] : α := 0 ↦ Λ 1, (#1)
+
+end combinator
+end pca
