src/re.lean
@@ -1,0 +1,180 @@
+import pca
+import combinator
+
+namespace pca
+
+universe variable u
+variables {α : Type u}
+
+namespace set
+
+inductive prec [pca α] (A : set α) : set α
+| rel {a} : a ∈ A → prec a
+| k : prec k
+| s : prec s
+| mul {a b c} : (↓a * ↓b) = ↓c → prec a → prec b → prec c
+notation `ℰ` := prec
+notation `ℰ₀` := prec ∅
+
+def recursive (A : set α) [pca α] : set α := {x | x ∈ prec A ∧ tot x}
+notation `ℛ` := recursive
+notation `ℛ₀` := recursive ∅
+
+lemma pr_subset [pca α] {A B : set α} {x : α} (hx : x ∈ ℰ A) (h : A ⊆ B) : x ∈ ℰ B :=
+begin
+  induction hx with a ha a b c e ha hb iha ihb,
+  { exact prec.rel (h ha),},
+  { exact prec.k, },
+  { exact prec.s, },
+  { exact prec.mul e iha ihb, },
+end
+
+lemma pr0_subset [pca α] {A : set α} {a : α} (ha : a ∈ (ℰ₀ : set α)) : a ∈ ℰ A :=
+pr_subset ha (by { simp, })
+
+lemma recuraive.k [pca α] (A : set α) : k ∈ ℛ A := ⟨prec.k, ktot⟩
+lemma recuraive.s [pca α] (A : set α) : s ∈ ℛ A := ⟨prec.s, stot⟩
+
+lemma prec.const (A : set α) [pca α] {a : α} : a ∈ (ℰ A : set α) → 𝐤 a ∈ (ℰ A : set α) :=
+begin
+  assume h : a ∈ ℰ A,
+  have l0 : ↓k * ↓a = ↓𝐤 a, { simp, },
+  show 𝐤 a ∈ ℰ A, from prec.mul l0 prec.k h,
+end
+
+lemma prec.subst [pca α] (A : set α) {a b : α} :
+  a ∈ ℰ A → b ∈ ℰ A → 𝐬 a b ∈ ℰ A :=
+begin
+  assume (ha : a ∈ ℰ A) (hb : b ∈ ℰ A),
+  have l0 : ↓s * ↓a = ↓𝐬' a, { unfold subst', simp, },
+  have l1 : 𝐬' a ∈ (ℰ A : set α), from prec.mul l0 prec.s ha,
+  have l2 : ↓𝐬' a * ↓b = ↓𝐬 a b, { unfold subst', simp, },
+  show 𝐬 a b ∈ ℰ A, from prec.mul l2 l1 hb,
+end
+
+lemma prec.i [pca α] {A : set α} : i ∈ ℰ A := prec.subst A prec.k prec.k
+lemma recursive.i [pca α] (A : set α) : i ∈ (ℛ A : set α) := ⟨prec.i, itot⟩
+
+inductive lambdar [pca α] (A : set α) 
+| var : ℕ → lambdar
+| com {a : α} : a ∈ ℰ A → lambdar
+| app : lambdar → lambdar → lambdar
+prefix `#₀`:max := lambdar.var
+prefix `&₀`:max := lambdar.com
+notation `k₀` := &₀prec.k
+notation `s₀` := &₀prec.s
+notation `i₀` := &₀prec.i
+instance lambdar_mul {A : set α} [pca α] : has_mul (lambdar A) := ⟨lambdar.app⟩
+
+def lamr [pca α] {A : set α} (n : ℕ) : lambdar A → lambdar A
+| #₀m     := if n = m then i₀ else k₀ * #₀m
+| &₀h     := k₀ * lambdar.com h
+| (l * m) := s₀ * (lamr l) * (lamr m)
+notation `Λ₀`x`,` := lamr x 
+
+def exprr [pca α] (A : set α): lambdar A → option α
+| #₀x := ↓k
+| (@lambdar.com _ _ _ e _) := ↓e
+| (l * m) := (exprr l) * (exprr m)
+
+lemma lambdar_defined [pca α] {A : set α} (n : ℕ) : ∀ (e : lambdar A), defined (exprr A (Λ₀ n, e))
+| #₀e := begin
+    cases (eq.decidable n e),
+    { simp[lamr, exprr, if_neg h], exact rfl, },
+    { simp[lamr, expr, if_pos h], exact rfl, },
+  end
+| (@lambdar.com _ _ _ e _) := ktot e
+| (l * m) := begin
+    simp [lamr, exprr], 
+    let a := option.get (lambdar_defined l),
+    let b := option.get (lambdar_defined m),
+    have ha : exprr A (Λ₀ n, l) = ↓a, { simp },
+    have hb : exprr A (Λ₀ n, m) = ↓b, { simp },
+    rw [ha, hb],
+    exact stot' a b
+  end
+
+notation n` -[`A`]→ ` l := option.get (@lambdar_defined _ _ A n l)
+
+lemma lambdar_pr [pca α] {A : set α} :
+  ∀ {e : lambdar A} (h : defined (exprr A e) = tt), option.get h ∈ (ℰ A : set α)
+| #₀_ _ := prec.k
+| &₀p _ := p
+| (l * m) h := begin
+    have ld : defined (exprr A l) = tt, from defined_l h,
+    have md : defined (exprr A m) = tt, from defined_r h,
+    have lpr : option.get ld ∈ ℰ A, from lambdar_pr ld,
+    have mpr : option.get md ∈ ℰ A, from lambdar_pr md,
+    have e : ↓option.get ld * ↓option.get md = ↓option.get h, { simp [exprr], },
+    show option.get h ∈ ℰ A, from prec.mul e lpr mpr,
+  end
+
+lemma lambda_pr0 [pca α] {A : set α} (n : ℕ) (e : lambdar A) : (n -[A]→ e) ∈ (ℰ A : set α) := lambdar_pr _
+
+namespace recursion_pr
+
+def d [pca α] : α := 0 -[∅]→ (Λ₀ 1, (#₀0 * #₀0 * #₀1))
+def dpr [pca α] : d ∈ (ℰ₀ : set α) := lambda_pr0 _ _
+
+def v [pca α]: α := 0 -[∅]→ (Λ₀ 1, (#₀0 * (&₀dpr * #₀1)))
+def vpr [pca α] : v ∈ (ℰ₀ : set α) := lambda_pr0 _ _
+
+def n [pca α] : α := 0 -[∅]→ (&₀dpr * (&₀vpr * #₀0))
+def npr [pca α] : n ∈ (ℰ₀ : set α) := lambda_pr0 _ _
+
+lemma fixpoint_eq_n [pca α] : @fixpoint α _ = n :=
+by { simp [fixpoint,recursion.n,n,recursion.d,recursion.v,d,v], refl, }
+
+lemma fixpoint_pr [pca α] : fixpoint ∈ (ℰ₀ : set α) := by { rw fixpoint_eq_n, exact npr, }
+lemma fixpoint_re [pca α] : fixpoint ∈ (ℛ₀ : set α) := ⟨fixpoint_pr, recursion.ntot⟩
+
+end recursion_pr
+
+class numbering (α : Type u) [pca α]
+(code : α → ℕ)
+(decode : ℕ → α)
+(nat_pr : ∀ n : ℕ, decode n ∈ (ℰ₀ : set α))
+(decode_code : ∀ x : α, x ∈ (ℰ₀ : set α) → decode (code x) = x)
+(code_decode : ∀ n : ℕ, code (decode n) = n)
+
+def Kl [pca α] : set α := {x : α | defined (↓x * ↓x)}
+def K (A : set α) [pca α] := {x : α | x ∈ A ∧ defined (↓x * ↓x)}
+def representable [pca α] (A : set α) : set (set α) := {B | ∃ e, e ∈ A ∧ B = {x | defined (↓e * ↓x)}}
+notation A` is_representable_in `B := A ∈ representable B
+def re_set [pca α] (A : set α) : Prop := ∃ e : α, e ∈ (ℰ₀ : set α) ∧ A = {x | defined (↓e * ↓x)}
+
+lemma neg_p_iff_negp (P : Prop) : ¬(P ↔ ¬P) := 
+begin
+  rintros ⟨h₀, h₁⟩,
+  have h₂ : ¬ P := λ p, h₀ p p,
+  exact h₂ (h₁ h₂),
+end
+
+lemma K_re [pca α] : Kl is_representable_in (ℰ₀ : set α) :=
+begin
+  use (0 ↦ #0 * #0),
+  have h : ∀ x : α, expr (Λ 0, (#0 * #0)) * ↓x = ↓x * ↓x, { intros x, simp [lam, expr], },
+  split,
+  { simp [lam, expr],
+    show 𝐬 i i ∈ ℰ₀, from prec.subst _ prec.i prec.i, },
+  apply set.ext,
+  intros x,
+  split,
+  { assume xK, simp, rw h x, exact xK, },
+  { unfold Kl, simp, assume xh, rw ← h x, exact xh, },
+end
+
+lemma compl_K_nre [pca α] : ¬ re_set (Klᶜ : set α) :=
+begin
+  rintro ⟨e, h⟩,
+  apply neg_p_iff_negp (e ∈ (Kl : set α)),
+  split,
+  { assume eK : e ∈ Kl,
+    show e ∈ (Klᶜ : set α), { rw h.2, simp, exact eK, }, },
+  { assume nKc : e ∉ Kl,
+    have eKc : e ∈ (Klᶜ : set α) := nKc,
+    show e ∈ Kl, { unfold Kl, simp, rw h.2 at eKc, exact eKc, }, },
+end
+
+end set
+end pca
